theories/Dot/typing_unstamped.v
@@ -1,0 +1,303 @@
+(**
+  An unstamped typing judgment for Dot, allowing only variables in paths, and not arbitrary values.
+  We show that unstamped typing derivations from here can
+  be converted to stamped derivations of this typing judgment, in lemma
+  [stamp_typing_mut].
+*)
+From D Require Import tactics.
+From D.Dot Require Export syn stampingDefsCore.
+
+Set Implicit Arguments.
+
+(* The typing judgement comes from [s/⊢/u⊢/] over [Dot/typing_objIdent.v], and dropping stamping. *)
+Reserved Notation "Γ u⊢ₜ e : T" (at level 74, e, T at next level).
+Reserved Notation "Γ u⊢ₚ p : T , i" (at level 74, p, T, i at next level).
+Reserved Notation "Γ |d V u⊢{ l := d  } : T" (at level 74, l, d, T, V at next level).
+Reserved Notation "Γ |ds V u⊢ ds : T" (at level 74, ds, T, V at next level).
+Reserved Notation "Γ u⊢ₜ T1 , i1 <: T2 , i2" (at level 74, T1, T2, i1, i2 at next level).
+
+Implicit Types (L T U V : ty) (v : vl) (e : tm) (d : dm) (p: path) (ds : dms) (Γ : list ty).
+
+(**
+Judgments for typing, subtyping, path and definition typing.
+*)
+Inductive typed Γ : tm → ty → Prop :=
+(** First, elimination forms *)
+(** Dependent application; only allowed if the argument is a value . *)
+| Appv_typed e1 x2 T1 T2:
+    Γ u⊢ₜ e1: TAll T1 T2 →                        Γ u⊢ₜ tv (var_vl x2) : T1 →
+    (*────────────────────────────────────────────────────────────*)
+    Γ u⊢ₜ tapp e1 (tv (var_vl x2)) : T2.|[(var_vl x2)/]
+(** Non-dependent application; allowed for any argument. *)
+| App_typed e1 e2 T1 T2:
+    Γ u⊢ₜ e1: TAll T1 T2.|[ren (+1)] →      Γ u⊢ₜ e2 : T1 →
+    (*────────────────────────────────────────────────────────────*)
+    Γ u⊢ₜ tapp e1 e2 : T2
+| Proj_typed e T l:
+    Γ u⊢ₜ e : TVMem l T →
+    (*─────────────────────────*)
+    Γ u⊢ₜ tproj e l : T
+| TMuE_typed x T:
+    Γ u⊢ₜ tv (var_vl x): TMu T →
+    (*──────────────────────*)
+    Γ u⊢ₜ tv (var_vl x): T.|[(var_vl x)/]
+(** Introduction forms *)
+| Lam_typed e T1 T2:
+    (* T1 :: Γ u⊢ₜ e : T2 → (* Would work, but allows the argument to occur in its own type. *) *)
+    is_unstamped_ty T1 →
+    nclosed T1 (length Γ) →
+    T1.|[ren (+1)] :: Γ u⊢ₜ e : T2 →
+    (*─────────────────────────*)
+    Γ u⊢ₜ tv (vabs e) : TAll T1 T2
+| VObj_typed ds T:
+    Γ |ds T u⊢ ds: T →
+    is_unstamped_ty T →
+    nclosed T (S (length Γ)) →
+    (*──────────────────────*)
+    Γ u⊢ₜ tv (vobj ds): TMu T
+| TMuI_typed x T:
+    Γ u⊢ₜ tv (var_vl x): T.|[(var_vl x)/] →
+    (*──────────────────────*)
+    Γ u⊢ₜ tv (var_vl x): TMu T
+| Nat_typed n:
+    Γ u⊢ₜ tv (vnat n): TNat
+
+(** "General" rules *)
+| Var_typed x T :
+    (* After looking up in Γ, we must weaken T for the variables on top of x. *)
+    Γ !! x = Some T →
+    (*──────────────────────*)
+    Γ u⊢ₜ tv (var_vl x) : T.|[ren (+x)]
+| Subs_typed e T1 T2 i :
+    Γ u⊢ₜ T1, 0 <: T2, i → Γ u⊢ₜ e : T1 →
+    (*───────────────────────────────*)
+    Γ u⊢ₜ iterate tskip i e : T2
+(* A bit surprising this is needed, but appears in the DOT papers, and this is
+   only admissible if t has a type U that is a proper subtype of TAnd T1 T2. *)
+| TAndI_typed T1 T2 x:
+    Γ u⊢ₜ tv (var_vl x) : T1 →
+    Γ u⊢ₜ tv (var_vl x) : T2 →
+    Γ u⊢ₜ tv (var_vl x) : TAnd T1 T2
+where "Γ u⊢ₜ e : T " := (typed Γ e T)
+with dms_typed Γ : ty → dms → ty → Prop :=
+| dnil_typed V : Γ |ds V u⊢ [] : TTop
+(* This demands definitions and members to be defined in aligned lists. *)
+| dcons_typed V l d ds T1 T2:
+    Γ |d V u⊢{ l := d } : T1 →
+    Γ |ds V u⊢ ds : T2 →
+    dms_hasnt ds l →
+    (*──────────────────────*)
+    Γ |ds V u⊢ (l, d) :: ds : TAnd T1 T2
+where "Γ |ds V u⊢ ds : T" := (dms_typed Γ V ds T)
+with dm_typed Γ : ty → label → dm → ty → Prop :=
+| dty_typed V l L T U:
+    nclosed T (S (length Γ)) →
+    is_unstamped_ty T →
+    TLater V :: Γ u⊢ₜ TLater L, 0 <: TLater T, 0 →
+    TLater V :: Γ u⊢ₜ TLater T, 0 <: TLater U, 0 →
+    Γ |d V u⊢{ l := dtysyn T } : TTMem l L U
+| dvl_typed V l v T:
+    V :: Γ u⊢ₜ tv v : T →
+    Γ |d V u⊢{ l := dvl v } : TVMem l T
+where "Γ |d V u⊢{ l := d  } : T" := (dm_typed Γ V l d T)
+with path_typed Γ : path → ty → nat → Prop :=
+| pv_typed x T:
+    Γ u⊢ₜ tv (var_vl x) : T →
+    Γ u⊢ₚ pv (var_vl x) : T, 0
+| pv_dlater p T i:
+    Γ u⊢ₚ p : TLater T, i →
+    Γ u⊢ₚ p : T, S i
+(* Mnemonic: Path from SELecting a Field *)
+| pself_typed p T i l:
+    Γ u⊢ₚ p : TVMem l T, i →
+    Γ u⊢ₚ pself p l : T, i
+| p_subs_typed p T1 T2 i j :
+    Γ u⊢ₜ T1, i <: T2, i + j →
+    Γ u⊢ₚ p : T1, i →
+    (*───────────────────────────────*)
+    Γ u⊢ₚ p : T2, i + j
+where "Γ u⊢ₚ p : T , i" := (path_typed Γ p T i)
+(* Γ u⊢ₜ T1, i1 <: T2, i2 means that TLater^i1 T1 <: TLater^i2 T2. *)
+with subtype Γ : ty → nat → ty → nat → Prop :=
+| Refl_stp i T :
+    is_unstamped_ty T →
+    nclosed T (length Γ) →
+    Γ u⊢ₜ T, i <: T, i
+| Trans_stp i1 i2 i3 T1 T2 T3:
+    Γ u⊢ₜ T1, i1 <: T2, i2 →
+    Γ u⊢ₜ T2, i2 <: T3, i3 →
+    Γ u⊢ₜ T1, i1 <: T3, i3
+| TLaterL_stp i T:
+    is_unstamped_ty T →
+    nclosed T (length Γ) →
+    Γ u⊢ₜ TLater T, i <: T, S i
+| TLaterR_stp i T:
+    is_unstamped_ty T →
+    nclosed T (length Γ) →
+    Γ u⊢ₜ T, S i <: TLater T, i
+
+(* "Structural" rules about indexes *)
+| TAddLater_stp T i:
+    is_unstamped_ty T →
+    nclosed T (length Γ) →
+    Γ u⊢ₜ T, i <: TLater T, i
+| TMono_stp T1 T2 i j:
+    Γ u⊢ₜ T1, i <: T2, j →
+    Γ u⊢ₜ T1, S i <: T2, S j
+
+(* "Logical" connectives *)
+| Top_stp i T :
+    is_unstamped_ty T →
+    nclosed T (length Γ) →
+    Γ u⊢ₜ T, i <: TTop, i
+| Bot_stp i T :
+    is_unstamped_ty T →
+    nclosed T (length Γ) →
+    Γ u⊢ₜ TBot, i <: T, i
+| TAnd1_stp T1 T2 i:
+    is_unstamped_ty T1 →
+    is_unstamped_ty T2 →
+    nclosed T1 (length Γ) →
+    nclosed T2 (length Γ) →
+    Γ u⊢ₜ TAnd T1 T2, i <: T1, i
+| TAnd2_stp T1 T2 i:
+    is_unstamped_ty T1 →
+    is_unstamped_ty T2 →
+    nclosed T1 (length Γ) →
+    nclosed T2 (length Γ) →
+    Γ u⊢ₜ TAnd T1 T2, i <: T2, i
+| TAnd_stp T U1 U2 i j:
+    Γ u⊢ₜ T, i <: U1, j →
+    Γ u⊢ₜ T, i <: U2, j →
+    Γ u⊢ₜ T, i <: TAnd U1 U2, j
+| TOr1_stp T1 T2 i:
+    is_unstamped_ty T1 →
+    is_unstamped_ty T2 →
+    nclosed T1 (length Γ) →
+    nclosed T2 (length Γ) →
+    Γ u⊢ₜ T1, i <: TOr T1 T2, i
+| TOr2_stp T1 T2 i:
+    is_unstamped_ty T1 →
+    is_unstamped_ty T2 →
+    nclosed T1 (length Γ) →
+    nclosed T2 (length Γ) →
+    Γ u⊢ₜ T2, i <: TOr T1 T2, i
+| TOr_stp T1 T2 U i j:
+    Γ u⊢ₜ T1, i <: U, j →
+    Γ u⊢ₜ T2, i <: U, j →
+    Γ u⊢ₜ TOr T1 T2, i <: U, j
+
+(* Type selections *)
+| SelU_stp l L U p i:
+    Γ u⊢ₚ p : TTMem l L U, i →
+    Γ u⊢ₜ TSel p l, i <: iterate TLater (S (plength p)) U, i
+| LSel_stp l L U p i:
+    Γ u⊢ₚ p : TTMem l L U, i →
+    Γ u⊢ₜ iterate TLater (S (plength p)) L, i <: TSel p l, i
+
+(* TODO: figure out if the drugs I had when I wrote these rules were good or bad. *)
+(* | SelU_stp l L U p i j: *)
+(*     Γ u⊢ₚ p : TTMem l L U, i → *)
+(*     Γ u⊢ₜ TSel p l, j <: U, S (i + j) *)
+(* | LSel_stp l L U p i j: *)
+(*     Γ u⊢ₚ p : TTMem l L U, i → *)
+(*     Γ u⊢ₜ L, S (i + j) <: TSel p l, j *)
+
+(* Subtyping for recursive types. Congruence, and opening in both directions. *)
+| Mu_stp_mu T1 T2 i:
+    (iterate TLater i T1 :: Γ) u⊢ₜ T1, i <: T2, i →
+    is_unstamped_ty T1 →
+    nclosed T1 (S (length Γ)) →
+    Γ u⊢ₜ TMu T1, i <: TMu T2, i
+| Mu_stp T i:
+    is_unstamped_ty T →
+    nclosed T (length Γ) →
+    Γ u⊢ₜ TMu T.|[ren (+1)], i <: T, i
+| Stp_mu T i:
+    is_unstamped_ty T →
+    nclosed T (length Γ) →
+    Γ u⊢ₜ T, i <: TMu T.|[ren (+1)], i
+
+(* "Congruence" or "variance" rules for subtyping. Unneeded for "logical" types.
+ "Cov" stands for covariance, "Con" for contravariance. *)
+(* Needed? Maybe drop later instead? *)
+| TLaterCov_stp T1 T2 i j:
+    Γ u⊢ₜ T1, S i <: T2, S j →
+    Γ u⊢ₜ TLater T1, i <: TLater T2, j
+| TAllConCov_stp T1 T2 U1 U2 i:
+    Γ u⊢ₜ TLater T2, i <: TLater T1, i →
+    iterate TLater (S i) T2.|[ren (+1)] :: Γ u⊢ₜ TLater U1, i <: TLater U2, i →
+    is_unstamped_ty T2 →
+    nclosed T2 (length Γ) →
+    Γ u⊢ₜ TAll T1 U1, i <: TAll T2 U2, i
+| TVMemCov_stp T1 T2 i l:
+    Γ u⊢ₜ TLater T1, i <: TLater T2, i →
+    Γ u⊢ₜ TVMem l T1, i <: TVMem l T2, i
+| TTMemConCov_stp L1 L2 U1 U2 i l:
+    Γ u⊢ₜ TLater L2, i <: TLater L1, i →
+    Γ u⊢ₜ TLater U1, i <: TLater U2, i →
+    Γ u⊢ₜ TTMem l L1 U1, i <: TTMem l L2 U2, i
+  (* Is it true that for covariant F, F[A ∧ B] = F[A] ∧ F[B]?
+    Dotty assumes that, tho DOT didn't capture it.
+    F[A ∧ B] <: F[A] ∧ F[B] is provable by covariance.
+    Let's prove F[A] ∧ F[B] <: F[A ∧ B] in the model.
+    *)
+| TAllDistr_stp T U1 U2 i:
+    is_unstamped_ty T →
+    is_unstamped_ty U1 →
+    is_unstamped_ty U2 →
+    nclosed T (length Γ) →
+    nclosed U1 (S (length Γ)) →
+    nclosed U2 (S (length Γ)) →
+    Γ u⊢ₜ TAnd (TAll T U1) (TAll T U2), i <: TAll T (TAnd U1 U2), i
+| TVMemDistr_stp l T1 T2 i:
+    is_unstamped_ty T1 →
+    is_unstamped_ty T2 →
+    nclosed T1 (length Γ) →
+    nclosed T2 (length Γ) →
+    Γ u⊢ₜ TAnd (TVMem l T1) (TVMem l T2), i <: TVMem l (TAnd T1 T2), i
+| TTMemDistr_strp l L U1 U2 i:
+    is_unstamped_ty L →
+    is_unstamped_ty U1 →
+    is_unstamped_ty U2 →
+    nclosed L (length Γ) →
+    nclosed U1 (length Γ) →
+    nclosed U2 (length Γ) →
+    Γ u⊢ₜ TAnd (TTMem l L U1) (TTMem l L U2), i <: TTMem l L (TAnd U1 U2), i
+where "Γ u⊢ₜ T1 , i1 <: T2 , i2" := (subtype Γ T1 i1 T2 i2).
+
+Scheme typed_mut_ind := Induction for typed Sort Prop
+with   dms_typed_mut_ind := Induction for dms_typed Sort Prop
+with   dm_typed_mut_ind := Induction for dm_typed Sort Prop
+with   path_typed_mut_ind := Induction for path_typed Sort Prop
+with   subtype_mut_ind := Induction for subtype Sort Prop.
+
+Combined Scheme typing_mut_ind from typed_mut_ind, dms_typed_mut_ind, dm_typed_mut_ind,
+  path_typed_mut_ind, subtype_mut_ind.
+
+Hint Constructors typed dms_typed dm_typed path_typed subtype.
+Remove Hints Trans_stp.
+Hint Extern 10 => try_once Trans_stp.
+
+Lemma unstamped_path_root_is_var Γ p T i:
+  Γ u⊢ₚ p : T, i → ∃ x, path_root p = var_vl x.
+Proof. by elim; intros; cbn; eauto 2. Qed.
+(*
+Section syntyping.
+  Context `{hasStampTable: stampTable}.
+  Lemma typing_obj_ident_to_typing Γ:
+    (∀ e T, Γ u⊢ₜ e : T → Γ ⊢ₜ e : T) ∧
+    (∀ V ds T, Γ |ds V u⊢ ds : T → Γ |ds V ⊢ ds : T) ∧
+    (∀ V l d T, Γ |d V u⊢{ l := d } : T → Γ |d V ⊢{ l := d } : T) ∧
+    (∀ p T i, Γ u⊢ₚ p : T, i → Γ ⊢ₚ p : T, i) ∧
+    (∀ T1 i1 T2 i2, Γ u⊢ₜ T1, i1 <: T2, i2 → Γ ⊢ₜ T1, i1 <: T2, i2).
+  Proof.
+    eapply typing_mut_ind with
+        (P := λ Γ e T _, Γ ⊢ₜ e : T)
+        (P0 := λ Γ V ds T _, Γ |ds V ⊢ ds : T)
+        (P1 := λ Γ V l d T _, Γ |d V ⊢{ l := d } : T)
+        (P2 := λ Γ p T i _, Γ ⊢ₚ p : T, i)
+        (P3 := λ Γ T1 i1 T2 i2 _, Γ ⊢ₜ T1, i1 <: T2, i2); clear Γ;
+      try solve [econstructor; eauto].
+  Qed.
+End syntyping. *)
